EvmCompiler/TypedCfg/Semantics.lean
@@ -138,45 +138,15 @@ def runPopMany : Nat → EVMState → Except EVMException EVMState
       runPopMany n state'
 
 def runDup (depth : Nat) (state : EVMState) : Except EVMException EVMState :=
-  match depth with
-  | 0 => Assembly.PrimOp.dup1.step state
-  | 1 => Assembly.PrimOp.dup2.step state
-  | 2 => Assembly.PrimOp.dup3.step state
-  | 3 => Assembly.PrimOp.dup4.step state
-  | 4 => Assembly.PrimOp.dup5.step state
-  | 5 => Assembly.PrimOp.dup6.step state
-  | 6 => Assembly.PrimOp.dup7.step state
-  | 7 => Assembly.PrimOp.dup8.step state
-  | 8 => Assembly.PrimOp.dup9.step state
-  | 9 => Assembly.PrimOp.dup10.step state
-  | 10 => Assembly.PrimOp.dup11.step state
-  | 11 => Assembly.PrimOp.dup12.step state
-  | 12 => Assembly.PrimOp.dup13.step state
-  | 13 => Assembly.PrimOp.dup14.step state
-  | 14 => Assembly.PrimOp.dup15.step state
-  | 15 => Assembly.PrimOp.dup16.step state
-  | _ => .error .InvalidInstruction
+  match dupOp? depth with
+  | some op => op.step state
+  | none => .error .InvalidInstruction
 
 def runSwap (depth : Nat) (state : EVMState) :
     Except EVMException EVMState :=
-  match depth with
-  | 0 => Assembly.PrimOp.swap1.step state
-  | 1 => Assembly.PrimOp.swap2.step state
-  | 2 => Assembly.PrimOp.swap3.step state
-  | 3 => Assembly.PrimOp.swap4.step state
-  | 4 => Assembly.PrimOp.swap5.step state
-  | 5 => Assembly.PrimOp.swap6.step state
-  | 6 => Assembly.PrimOp.swap7.step state
-  | 7 => Assembly.PrimOp.swap8.step state
-  | 8 => Assembly.PrimOp.swap9.step state
-  | 9 => Assembly.PrimOp.swap10.step state
-  | 10 => Assembly.PrimOp.swap11.step state
-  | 11 => Assembly.PrimOp.swap12.step state
-  | 12 => Assembly.PrimOp.swap13.step state
-  | 13 => Assembly.PrimOp.swap14.step state
-  | 14 => Assembly.PrimOp.swap15.step state
-  | 15 => Assembly.PrimOp.swap16.step state
-  | _ => .error .InvalidInstruction
+  match swapOp? depth with
+  | some op => op.step state
+  | none => .error .InvalidInstruction
 
 def run (instr : Instr) (state : EVMState) : Except EVMException EVMState :=
   match instr with
